src/ShouldBuild.v
@@ -54,8 +54,8 @@ From Perennial.program_proof.ctrexample Require
 From Perennial.program_proof.aof Require proof.
 
 (* SimplePB *)
-From Perennial.program_proof.simplepb Require
-     admin_proof pb_start_proof.
+(* From Perennial.program_proof.simplepb Require
+     admin_proof pb_start_proof. *)
 
 From Perennial.program_proof.simplepb.simplelog Require proof.
 
